Classical_Grounding/Planner_Export.thy
@@ -21,7 +21,7 @@ export_code
   plan_by_cert_dfs ground_via_cert'_dfs ground_via_cert_dfs
   ground_via_cert_numeric_dfs_e ground_via_cert_numeric_exec_e ground_via_cert_numeric_gdfs_e
   ground_via_cert_numeric_dfs_stream_e ground_via_cert_numeric_exec_stream_e ground_via_cert_numeric_gdfs_stream_e
-  ast_classical_problem.P\<^sub>T cert_ops_of_exec_fast canon ast_classical_problem.varfree_ground_ac
+  ast_classical_problem.P\<^sub>T cert_ops_of_exec_fast canon ast_classical_problem.varfree_inst_ac
   distinct_strings_lit varfree.op_names
   ground_via_cert_prop_dfs_e
   dl_program_of sat_solve_strips
